
2. ∂C/∂A(2) = 2 * (A(2) - Y) / Nout

3. ∂C/∂Z(2) = ∂C/∂A(2) * ∂A(2)/∂Z(2)  
   ∂C/∂Z(2) = ∂C/∂A(2) * σ'(Z(2))
   ∂C/∂Z(2) = ∂C/∂A(2) * σ(Z(2)) * (1-σ(Z(2)))
   ∂C/∂Z(2) = ∂C/∂A(2) * A(2) * (1 - A(2))

4. ∂C/∂W(2) = ∂C/∂Z(2) * ∂Z(2)/∂W(2)
   ∂C/∂W(2) = ∂C/∂Z(2) * A(1)

5. ∂C/∂B(2) = ∂C/∂Z(2) * ∂Z(2)/∂B(2)
   ∂C/∂B(2) = sum(∂C/∂Z(2), axis=0)

6. ∂C/∂A(1) = ∂C/∂Z(2) * ∂Z(2)/∂A(1)
   ∂C/∂A(1) = ∂C/∂Z(2) * W(2)

7. ∂C/∂Z(1) = ∂C/∂A(1) * σ'(Z(1))
   ∂C/∂Z(1) = ∂C/∂A(1) * A(1) * (1 - A(1))

8. ∂C/∂W(1) = ∂C/∂Z(1) * A(0)

9. ∂C/∂B(1) = sum(∂C/∂Z(1), axis=0)

